\documentclass[a4paper,12pt]{article}
\begin{document}
\vspace{30pt}
\begin{eqnarray*}
\delta = (a(k + 1) - \alpha \hat{a})^2 \\
a(k+1) = a(k) + y_k \\
\delta = ||a(k) - \alpha \hat{a}||^2 + 2 ( a(k) - \alpha \hat{a} )^ty_k + ||y_k||^2 \\
\delta \leq ||a(k) - \alpha \hat{a}||^2 - 2\alpha \hat{a}^ty_k + ||y_k||^2 \\
\beta^2 = max_i y^2     \forall i \\
\Omega  = min [\hat{a} y_k] \forall y_k \in datasamples\\
\delta \leq ||a(k) - \alpha \hat{a}||^2 - 2\alpha \Omega + \beta^2 \\
\alpha = \beta^2 / \Omega \\
\delta = ||a(k) - \alpha \hat{a}||^2 - \beta^2 \\
(a(k + 1) - \alpha \hat{a})^2 \leq (a(k + 1) - \alpha \hat{a})^2 -\beta^2\\
k_0=\frac{||a(1) - \alpha \hat{a}||^2}{\beta^2}\\
\end{eqnarray*}
\end{document}